\chapter{Logic}
\begin{defn}
Proposition is a statement that is either true or false, but not both.
\end{defn}

\section{Logical operations}
\subsection{Definition of $\lnot$}
\begin{defn}
\label{Definition:lnot_True}
\begin{align*}
& \lnot (\text{True}) \\
\overset{\operatorname{def}}{\iff} & \text{False}
\end{align*}
\end{defn}

\begin{defn}
\label{Definition:lnot_False}
\begin{align*}
& \lnot (\text{False}) \\
\overset{\operatorname{def}}{\iff} & \text{True}
\end{align*}
\end{defn}

\subsection{Definition of $\lor$}
\begin{defn}
\label{Definition:lor_True_True}
\begin{align*}
& (\text{True}) \lor (\text{True}) \\
\overset{\operatorname{def}}{\iff} & \text{True}
\end{align*}
\end{defn}

\begin{defn}
\label{Definition:lor_True_False}
\begin{align*}
& (\text{True}) \lor (\text{False}) \\
\overset{\operatorname{def}}{\iff} & \text{True}
\end{align*}
\end{defn}

\begin{defn}
\label{Definition:lor_False_True}
\begin{align*}
& (\text{False}) \lor (\text{True}) \\
\overset{\operatorname{def}}{\iff} & \text{True}
\end{align*}
\end{defn}

\begin{defn}
\label{Definition:lor_False_False}
\begin{align*}
& (\text{False}) \lor (\text{False}) \\
\overset{\operatorname{def}}{\iff} & \text{False}
\end{align*}
\end{defn}

\subsection{Definition of $\land$}
\begin{defn}
\label{Definition:land_True_True}
\begin{align*}
& (\text{True}) \land (\text{True}) \\
\overset{\operatorname{def}}{\iff} & \text{True}
\end{align*}
\end{defn}

\begin{defn}
\label{Definition:land_True_False}
\begin{align*}
& (\text{True}) \land (\text{False}) \\
\overset{\operatorname{def}}{\iff} & \text{False}
\end{align*}
\end{defn}

\begin{defn}
\label{Definition:land_False_True}
\begin{align*}
& (\text{False}) \land (\text{True}) \\
\overset{\operatorname{def}}{\iff} & \text{False}
\end{align*}
\end{defn}

\begin{defn}
\label{Definition:land_False_False}
\begin{align*}
& (\text{False}) \land (\text{False}) \\
\overset{\operatorname{def}}{\iff} & \text{False}
\end{align*}
\end{defn}

\subsection{Definition of $\iff$}
\begin{defn}
\label{Definition:iff}
\begin{align*}
& a \iff b \\
\overset{\operatorname{def}}{\iff} & (a \land b) \lor ((\lnot a) \land (\lnot b))
\end{align*}
\end{defn}

\subsection{Definition of $\implies$}
\begin{defn}
\label{Definition:implies}
\begin{align*}
& a \implies b \\
\overset{\operatorname{def}}{\iff} & (\lnot a) \lor b
\end{align*}
\end{defn}

\section{Boolean algebra}
\subsection{Associativity of $\lor$}
\begin{prop}
\label{Proposition:lor_associativity}
\begin{align*}
& (a \lor b) \lor c \\
\iff & a \lor (b \lor c)
\end{align*}
\end{prop}

\subsection{Associativity of $\land$}
\begin{prop}
\label{Proposition:land_associativity}
\begin{align*}
& (a \land b) \land c \\
\iff & a \land (b \land c)
\end{align*}
\end{prop}

\subsection{Commutativity of $\lor$}
\begin{prop}
\label{Proposition:lor_commutativity}
\begin{align*}
& a \lor b \\
\iff & b \lor a
\end{align*}
\end{prop}

\subsection{Commutativity of $\land$}
\begin{prop}
\label{Proposition:land_commutativity}
\begin{align*}
& a \land b \\
\iff & b \land a
\end{align*}
\end{prop}

\subsection{Identity of $\lor$}
\begin{prop}
\label{Proposition:lor_identity_1}
\begin{align*}
& a \lor (\text{False}) \\
\iff & a
\end{align*}
\end{prop}

\begin{prop}
\label{Proposition:lor_identity_2}
\begin{align*}
& (\text{False}) \lor a \\
\iff & a
\end{align*}
\end{prop}

\subsection{Identity of $\land$}
\begin{prop}
\label{Proposition:land_identity_1}
\begin{align*}
& a \land (\text{True}) \\
\iff & a
\end{align*}
\end{prop}

\begin{prop}
\label{Proposition:land_identity_2}
\begin{align*}
& (\text{True}) \land a \\
\iff & a
\end{align*}
\end{prop}

\subsection{Annihilator of $\lor$}
\begin{prop}
\label{Proposition:lor_annihilator_1}
\begin{align*}
& a \lor (\text{True}) \\
\iff & \text{True}
\end{align*}
\end{prop}

\begin{prop}
\label{Proposition:lor_annihilator_2}
\begin{align*}
& (\text{True}) \lor a \\
\iff & \text{True}
\end{align*}
\end{prop}

\subsection{Annihilator of $\land$}
\begin{prop}
\label{Proposition:land_annihilator_1}
\begin{align*}
& a \land (\text{False}) \\
\iff & \text{False}
\end{align*}
\end{prop}

\begin{prop}
\label{Proposition:land_annihilator_2}
\begin{align*}
& (\text{False}) \land a \\
\iff & \text{False}
\end{align*}
\end{prop}

\subsection{Idempotence of $\lor$}
\begin{prop}
\label{Proposition:lor_idempotence}
\begin{align*}
& a \lor a \\
\iff & a
\end{align*}
\end{prop}

\subsection{Idempotence of $\land$}
\begin{prop}
\label{Proposition:land_idempotence}
\begin{align*}
& a \land a \\
\iff & a
\end{align*}
\end{prop}

\subsection{Complement of $\lor$}
\begin{prop}
\label{Proposition:lor_complement_1}
\begin{align*}
& a \lor (\lnot a) \\
\iff & \text{True}
\end{align*}
\end{prop}

\begin{prop}
\label{Proposition:lor_complement_2}
\begin{align*}
& (\lnot a) \lor a \\
\iff & \text{True}
\end{align*}
\end{prop}

\subsection{Complement of $\land$}
\begin{prop}
\label{Proposition:land_complement_1}
\begin{align*}
& a \land (\lnot a) \\
\iff & \text{False}
\end{align*}
\end{prop}

\begin{prop}
\label{Proposition:land_complement_2}
\begin{align*}
& (\lnot a) \land a \\
\iff & \text{False}
\end{align*}
\end{prop}

\subsection{Absorption of $\lor$ over $\land$}
\begin{prop}
\label{Proposition:lor_land_absorption_1}
\begin{align*}
& a \lor (a \land b) \\
\iff & a
\end{align*}
\end{prop}

\begin{prop}
\label{Proposition:lor_land_absorption_2}
\begin{align*}
& a \lor (b \land a) \\
\iff & a
\end{align*}
\end{prop}

\begin{prop}
\label{Proposition:lor_land_absorption_3}
\begin{align*}
& (a \land b) \lor a \\
\iff & a
\end{align*}
\end{prop}

\begin{prop}
\label{Proposition:lor_land_absorption_4}
\begin{align*}
& (b \land a) \lor a \\
\iff & a
\end{align*}
\end{prop}

\subsection{Absorption of $\land$ over $\lor$}
\begin{prop}
\label{Proposition:land_lor_absorption_1}
\begin{align*}
& a \land (a \lor b) \\
\iff & a
\end{align*}
\end{prop}

\begin{prop}
\label{Proposition:land_lor_absorption_2}
\begin{align*}
& a \land (b \lor a) \\
\iff & a
\end{align*}
\end{prop}

\begin{prop}
\label{Proposition:land_lor_absorption_3}
\begin{align*}
& (a \lor b) \land a \\
\iff & a
\end{align*}
\end{prop}

\begin{prop}
\label{Proposition:land_lor_absorption_4}
\begin{align*}
& (b \lor a) \land a \\
\iff & a
\end{align*}
\end{prop}

\subsection{Distributivity of $\lor$ over $\land$}
\begin{prop}
\label{Proposition:lor_land_distributivity_1}
\begin{align*}
& a \lor (b \land c) \\
\iff & (a \lor b) \land (a \lor c)
\end{align*}
\end{prop}

\begin{prop}
\label{Proposition:lor_land_distributivity_2}
\begin{align*}
& (a \land b) \lor c \\
\iff & (a \lor c) \land (b \lor c)
\end{align*}
\end{prop}

\subsection{Distributivity of $\land$ over $\lor$}
\begin{prop}
\label{Proposition:land_lor_distributivity_1}
\begin{align*}
& a \land (b \lor c) \\
\iff & (a \land b) \lor (a \land c)
\end{align*}
\end{prop}

\begin{prop}
\label{Proposition:land_lor_distributivity_2}
\begin{align*}
& (a \lor b) \land c \\
\iff & (a \land c) \lor (b \land c)
\end{align*}
\end{prop}

\subsection{Double negation}
\begin{prop}
\label{Proposition:double_negation}
\begin{align*}
& \lnot (\lnot a) \\
\iff & a
\end{align*}
\end{prop}

\subsection{De Morgan's laws}
\begin{prop}
\label{Proposition:De_Morgan_lor}
\begin{align*}
& \lnot (a \lor b) \\
\iff & (\lnot a) \land (\lnot b)
\end{align*}
\end{prop}

\begin{prop}
\label{Proposition:De_Morgan_land}
\begin{align*}
& \lnot (a \land b) \\
\iff & (\lnot a) \lor (\lnot b)
\end{align*}
\end{prop}

\section{Basic Proposition}
\begin{prop}
\label{Proposition:a_lor_b_complement}
\begin{align*}
& (a \land (\lnot b)) \lor b \\
\iff & a \lor b
\end{align*}
Proof of Proposition \ref{Proposition:a_lor_b_complement}
\begin{align*}
& (a \land (\lnot b)) \lor b \\
\iff & (a \lor b) \land ((\lnot b) \lor b)
&& \text{Proposition \ref{Proposition:lor_land_distributivity_2}} \\
\iff & (a \lor b) \land (\text{True})
&& \text{Proposition \ref{Proposition:lor_complement_2}} \\
\iff & a \lor b
&& \text{Proposition \ref{Proposition:land_identity_1}} \\
\end{align*}
\end{prop}

\section{Proof technique}
\begin{prop}
\label{Proposition:true_statement}
\begin{align*}
& a \iff (\text{True}) \\
\iff & a
\end{align*}
Proof of Proposition \ref{Proposition:true_statement}
\begin{align*}
& a \iff (\text{True}) \\
\overset{\operatorname{def}}{\iff} & (a \land (\text{True})) \lor ((\lnot a) \land (\lnot (\text{True})))
&& \text{Definition \ref{Definition:iff}} \\
\overset{\operatorname{def}}{\iff} & (a \land (\text{True})) \lor ((\lnot a) \land (\text{False}))
&& \text{Definition \ref{Definition:lnot_True}} \\
\iff & a \lor ((\lnot a) \land (\text{False}))
&& \text{Proposition \ref{Proposition:land_identity_1}} \\
\iff & a \lor (\text{False})
&& \text{Proposition \ref{Proposition:land_annihilator_1}} \\
\iff & a
&& \text{Proposition \ref{Proposition:lor_identity_1}} \\
\end{align*}
\end{prop}

\begin{prop}
\label{Proposition:implies_lor}
\begin{align*}
& a \implies b \\
\implies & (a \lor c) \implies (b \lor c)
\end{align*}
Proof of Proposition \ref{Proposition:implies_lor}
\begin{align*}
& (a \implies b) \implies ((a \lor c) \implies (b \lor c)) \\
\overset{\operatorname{def}}{\iff} & ((\lnot a) \lor b) \implies ((a \lor c) \implies (b \lor c))
&& \text{Definition \ref{Definition:implies}} \\
\overset{\operatorname{def}}{\iff} & ((\lnot a) \lor b) \implies ((\lnot (a \lor c)) \lor (b \lor c))
&& \text{Definition \ref{Definition:implies}} \\
\overset{\operatorname{def}}{\iff} & (\lnot ((\lnot a) \lor b)) \lor ((\lnot (a \lor c)) \lor (b \lor c))
&& \text{Definition \ref{Definition:implies}} \\
\iff & ((\lnot (\lnot a)) \land (\lnot b)) \lor ((\lnot (a \lor c)) \lor (b \lor c))
&& \text{Proposition \ref{Proposition:De_Morgan_lor}} \\
\iff & (a \land (\lnot b)) \lor ((\lnot (a \lor c)) \lor (b \lor c))
&& \text{Proposition \ref{Proposition:double_negation}} \\
\iff & (a \land (\lnot b)) \lor (((\lnot a) \land (\lnot c)) \lor (b \lor c))
&& \text{Proposition \ref{Proposition:De_Morgan_lor}} \\
\iff & (a \land (\lnot b)) \lor (((\lnot a) \land (\lnot c)) \lor (c \lor b))
&& \text{Proposition \ref{Proposition:lor_commutativity}} \\
\iff & (a \land (\lnot b)) \lor ((((\lnot a) \land (\lnot c)) \lor c) \lor b)
&& \text{Proposition \ref{Proposition:lor_associativity}} \\
\iff & (a \land (\lnot b)) \lor (b \lor (((\lnot a) \land (\lnot c)) \lor c))
&& \text{Proposition \ref{Proposition:lor_commutativity}} \\
\iff & ((a \land (\lnot b)) \lor b) \lor (((\lnot a) \land (\lnot c)) \lor c)
&& \text{Proposition \ref{Proposition:lor_associativity}} \\
\iff & (a \lor b) \lor (((\lnot a) \land (\lnot c)) \lor c)
&& \text{Proposition \ref{Proposition:a_lor_b_complement}} \\
\iff & (a \lor b) \lor ((\lnot a) \lor c)
&& \text{Proposition \ref{Proposition:a_lor_b_complement}} \\
\iff & ((a \lor b) \lor (\lnot a)) \lor c
&& \text{Proposition \ref{Proposition:lor_associativity}} \\
\iff & ((\lnot a) \lor (a \lor b)) \lor c
&& \text{Proposition \ref{Proposition:lor_commutativity}} \\
\iff & (((\lnot a) \lor a) \lor b) \lor c
&& \text{Proposition \ref{Proposition:lor_associativity}} \\
\iff & ((\text{True}) \lor b) \lor c
&& \text{Proposition \ref{Proposition:lor_complement_2}} \\
\iff & (\text{True}) \lor c
&& \text{Proposition \ref{Proposition:lor_annihilator_2}} \\
\iff & \text{True}
&& \text{Proposition \ref{Proposition:lor_annihilator_2}} \\
\end{align*}
\end{prop}

\begin{prop}
\label{Proposition:implies_land}
\begin{align*}
& a \implies b \\
\implies & (a \land c) \implies (b \land c)
\end{align*}
\end{prop}

\begin{prop}
\label{Proposition:contrapositive}
Contrapositive
\begin{align*}
& a \implies b \\
\iff & (\lnot b) \implies (\lnot a)
\end{align*}
\end{prop}

\begin{prop}
\label{Proposition:implies_transitive}
Transitive property of $\implies$.
\begin{align*}
& (a \implies b) \land (b \implies c) \\
\implies & a \implies c
\end{align*}
\end{prop}

\begin{prop}
\label{Proposition:iff_implies}
\begin{align*}
& a \iff b \\
\iff & (a \implies b) \land (b \implies a)
\end{align*}
\end{prop}

\begin{prop}
\label{Proposition:iff_lor}
\begin{align*}
& a \iff b \\
\implies & (a \lor c) \iff (b \lor c)
\end{align*}
\end{prop}

\begin{prop}
\label{Proposition:iff_land}
\begin{align*}
& a \iff b \\
\implies & (a \land c) \iff (b \land c)
\end{align*}
\end{prop}

\begin{prop}
\label{Proposition:iff_symmetric}
Symmetric property of $\iff$.
\begin{align*}
& a \iff b \\
\iff & b \iff a
\end{align*}
\end{prop}

\begin{prop}
\label{Proposition:iff_contrapositive}
\begin{align*}
& a \iff b \\
\iff & (\lnot a) \iff (\lnot b)
\end{align*}
\end{prop}

\begin{prop}
\label{Proposition:iff_transitive}
Transitive property of $\iff$.
\begin{align*}
& (a \iff b) \land (b \iff c) \\
\implies & a \iff c
\end{align*}
\end{prop}

\begin{prop}
\label{Proposition:iff_reflexive}
Reflexive property of $\iff$.
\begin{align*}
& a \\
\iff & a
\end{align*}
Proof of Proposition \ref{Proposition:iff_reflexive}
\begin{align*}
& a \iff a \\
\overset{\operatorname{def}}{\iff} & (a \land a) \lor ((\lnot a) \land (\lnot a))
&& \text{Definition \ref{Definition:iff}} \\
\iff & a \lor ((\lnot a) \land (\lnot a))
&& \text{Proposition \ref{Proposition:land_idempotence}} \\
\iff & a \lor (\lnot a)
&& \text{Proposition \ref{Proposition:land_idempotence}} \\
\iff & \text{True}
&& \text{Proposition \ref{Proposition:lor_complement_1}} \\
\end{align*}
\end{prop}

\section{Quantifiers}
\begin{defn}
Universal quantifier is denoted by $\forall$.
\begin{align*}
& \forall x (P(x)) \\
\overset{\operatorname{def}}{\iff} & (P(x_1) \land P(x_2) \land \dots)
\end{align*}
\end{defn}

\begin{defn}
Existential quantifier is denoted by $\exists$.
\begin{align*}
& \exists x (P(x)) \\
\overset{\operatorname{def}}{\iff} & (P(x_1) \lor P(x_2) \lor \dots)
\end{align*}
\end{defn}

\begin{prop}
\label{Proposition:forall_land_commutativity}
\begin{align*}
& \forall x (P(x) \land Q(x)) \\
\iff & (\forall x (P(x))) \land (\forall x (Q(x)))
\end{align*}
\end{prop}

\begin{prop}
\label{Proposition:exists_lor_commutativity}
\begin{align*}
& \exists x (P(x) \lor Q(x)) \\
\iff & (\exists x (P(x))) \lor (\exists x (Q(x)))
\end{align*}
\end{prop}

\begin{prop}
\label{Proposition:lor_forall_distributivity}
\begin{align*}
& P \lor (\forall x (Q(x))) \\
\iff & \forall x (P \lor (Q(x)))
\end{align*}
\end{prop}

\begin{prop}
\label{Proposition:land_exists_distributivity}
\begin{align*}
& P \land (\exists x (Q(x))) \\
\iff & \exists x (P \land (Q(x)))
\end{align*}
\end{prop}

\begin{axm}
\label{Axiom:forall_independent_variable}
\begin{align*}
& \forall x (P(y)) \\
\iff & P(y)
\end{align*}
\end{axm}

\begin{axm}
\label{Axiom:exists_independent_variable}
\begin{align*}
& \exists x (P(y)) \\
\iff & P(y)
\end{align*}
\end{axm}

\begin{axm}
\label{Axiom:De_Morgan_1}
De Morgan's law
\begin{align*}
& \lnot (\forall x (P(x))) \\
\iff & \exists x (\lnot (P(x)))
\end{align*}
\end{axm}

\begin{axm}
\label{Axiom:De_Morgan_2}
De Morgan's law
\begin{align*}
& \lnot (\exists x (P(x))) \\
\iff & \forall x (\lnot (P(x)))
\end{align*}
\end{axm}

\begin{defn}
\label{Definition:uniqueness_quantifier}
Uniqueness quantifier is denoted by $!\exists$.
\begin{align*}
& !\exists x (P(x)) \\
\overset{\operatorname{def}}{\iff} & (\exists x (P(x))) \land (\forall x \forall y ((P(x) \land P(y)) \implies (x = y)))
\end{align*}
\end{defn}

\begin{axm}
\label{Axiom:axiom_of_substitution}
Axiom of Substitution
\begin{align*}
\forall x ((\exists y ((y = x) \land P(y))) \iff P(x))
\end{align*}
\end{axm}

\section{Logic proposition}
\begin{prop}
\label{Proposition:land_implies_iff}
\begin{align*}
& a \land b \\
\implies & a \iff b
\end{align*}
\end{prop}

\begin{prop}
\label{Proposition:land_omit}
\begin{align*}
& a \land b \\
\implies & a
\end{align*}
\end{prop}

\begin{prop}
\label{Proposition:lemma_uniqueness}
\begin{align*}
& a \land ((b \land a) \implies c) \\
\implies & b \implies c
\end{align*}
\end{prop}

\begin{prop}
\label{Proposition:implies_satisfy}
\begin{align*}
& a \land (a \implies b) \\
\implies & b
\end{align*}
\end{prop}

\begin{prop}
\label{Proposition:iff_satisfy}
\begin{align*}
& a \land (a \iff b) \\
\implies & b
\end{align*}
\end{prop}

