\chapter{Logic}
\begin{defn}
Proposition is a statement that is either true or false, but not both.
\end{defn}

\section{Logical operations}
\subsection{Definition of $\lnot$}
\begin{defn}
\label{Definition:lnot_True}
\begin{align*}
& \lnot (\text{True}) \\
\overset{\operatorname{def}}{\iff} & \text{False}
\end{align*}
\end{defn}

\begin{defn}
\label{Definition:lnot_False}
\begin{align*}
& \lnot (\text{False}) \\
\overset{\operatorname{def}}{\iff} & \text{True}
\end{align*}
\end{defn}

\subsection{Definition of $\lor$}
\begin{defn}
\label{Definition:lor_True_True}
\begin{align*}
& (\text{True}) \lor (\text{True}) \\
\overset{\operatorname{def}}{\iff} & \text{True}
\end{align*}
\end{defn}

\begin{defn}
\label{Definition:lor_True_False}
\begin{align*}
& (\text{True}) \lor (\text{False}) \\
\overset{\operatorname{def}}{\iff} & \text{True}
\end{align*}
\end{defn}

\begin{defn}
\label{Definition:lor_False_True}
\begin{align*}
& (\text{False}) \lor (\text{True}) \\
\overset{\operatorname{def}}{\iff} & \text{True}
\end{align*}
\end{defn}

\begin{defn}
\label{Definition:lor_False_False}
\begin{align*}
& (\text{False}) \lor (\text{False}) \\
\overset{\operatorname{def}}{\iff} & \text{False}
\end{align*}
\end{defn}

\subsection{Definition of $\land$}
\begin{defn}
\label{Definition:land_True_True}
\begin{align*}
& (\text{True}) \land (\text{True}) \\
\overset{\operatorname{def}}{\iff} & \text{True}
\end{align*}
\end{defn}

\begin{defn}
\label{Definition:land_True_False}
\begin{align*}
& (\text{True}) \land (\text{False}) \\
\overset{\operatorname{def}}{\iff} & \text{False}
\end{align*}
\end{defn}

\begin{defn}
\label{Definition:land_False_True}
\begin{align*}
& (\text{False}) \land (\text{True}) \\
\overset{\operatorname{def}}{\iff} & \text{False}
\end{align*}
\end{defn}

\begin{defn}
\label{Definition:land_False_False}
\begin{align*}
& (\text{False}) \land (\text{False}) \\
\overset{\operatorname{def}}{\iff} & \text{False}
\end{align*}
\end{defn}

\subsection{Definition of $\iff$}
\begin{defn}
\label{Definition:iff}
\begin{align*}
& x \iff y \\
\overset{\operatorname{def}}{\iff} & (x \land y) \lor ((\lnot x) \land (\lnot y))
\end{align*}
\end{defn}

\subsection{Definition of $\implies$}
\begin{defn}
\label{Definition:implies}
\begin{align*}
& x \implies y \\
\overset{\operatorname{def}}{\iff} & (\lnot x) \lor y
\end{align*}
\end{defn}

\section{Boolean algebra}
\subsection{Associativity of $\lor$}
\begin{prop}
\label{Proposition:lor_associativity}
\begin{align*}
& (x \lor y) \lor z \\
\iff & x \lor (y \lor z)
\end{align*}
\end{prop}

\subsection{Associativity of $\land$}
\begin{prop}
\label{Proposition:land_associativity}
\begin{align*}
& (x \land y) \land z \\
\iff & x \land (y \land z)
\end{align*}
\end{prop}

\subsection{Commutativity of $\lor$}
\begin{prop}
\label{Proposition:lor_commutativity}
\begin{align*}
& x \lor y \\
\iff & y \lor x
\end{align*}
\end{prop}

\subsection{Commutativity of $\land$}
\begin{prop}
\label{Proposition:land_commutativity}
\begin{align*}
& x \land y \\
\iff & y \land x
\end{align*}
\end{prop}

\subsection{Identity of $\lor$}
\begin{prop}
\label{Proposition:lor_identity_1}
\begin{align*}
& x \lor (\text{False}) \\
\iff & x
\end{align*}
\end{prop}

\begin{prop}
\label{Proposition:lor_identity_2}
\begin{align*}
& (\text{False}) \lor x \\
\iff & x
\end{align*}
\end{prop}

\subsection{Identity of $\land$}
\begin{prop}
\label{Proposition:land_identity_1}
\begin{align*}
& x \land (\text{True}) \\
\iff & x
\end{align*}
\end{prop}

\begin{prop}
\label{Proposition:land_identity_2}
\begin{align*}
& (\text{True}) \land x \\
\iff & x
\end{align*}
\end{prop}

\subsection{Annihilator of $\lor$}
\begin{prop}
\label{Proposition:lor_annihilator_1}
\begin{align*}
& x \lor (\text{True}) \\
\iff & \text{True}
\end{align*}
\end{prop}

\begin{prop}
\label{Proposition:lor_annihilator_2}
\begin{align*}
& (\text{True}) \lor x \\
\iff & \text{True}
\end{align*}
\end{prop}

\subsection{Annihilator of $\land$}
\begin{prop}
\label{Proposition:land_annihilator_1}
\begin{align*}
& x \land (\text{False}) \\
\iff & \text{False}
\end{align*}
\end{prop}

\begin{prop}
\label{Proposition:land_annihilator_2}
\begin{align*}
& (\text{False}) \land x \\
\iff & \text{False}
\end{align*}
\end{prop}

\subsection{Idempotence of $\lor$}
\begin{prop}
\label{Proposition:lor_idempotence}
\begin{align*}
& x \lor x \\
\iff & x
\end{align*}
\end{prop}

\subsection{Idempotence of $\land$}
\begin{prop}
\label{Proposition:land_idempotence}
\begin{align*}
& x \land x \\
\iff & x
\end{align*}
\end{prop}

\subsection{Complement of $\lor$}
\begin{prop}
\label{Proposition:lor_complement_1}
\begin{align*}
& x \lor (\lnot x) \\
\iff & \text{True}
\end{align*}
\end{prop}

\begin{prop}
\label{Proposition:lor_complement_2}
\begin{align*}
& (\lnot x) \lor x \\
\iff & \text{True}
\end{align*}
\end{prop}

\subsection{Complement of $\land$}
\begin{prop}
\label{Proposition:land_complement_1}
\begin{align*}
& x \land (\lnot x) \\
\iff & \text{False}
\end{align*}
\end{prop}

\begin{prop}
\label{Proposition:land_complement_2}
\begin{align*}
& (\lnot x) \land x \\
\iff & \text{False}
\end{align*}
\end{prop}

\subsection{Absorption of $\lor$ over $\land$}
\begin{prop}
\label{Proposition:lor_land_absorption_1}
\begin{align*}
& x \lor (x \land y) \\
\iff & x
\end{align*}
\end{prop}

\begin{prop}
\label{Proposition:lor_land_absorption_2}
\begin{align*}
& x \lor (y \land x) \\
\iff & x
\end{align*}
\end{prop}

\begin{prop}
\label{Proposition:lor_land_absorption_3}
\begin{align*}
& (x \land y) \lor x \\
\iff & x
\end{align*}
\end{prop}

\begin{prop}
\label{Proposition:lor_land_absorption_4}
\begin{align*}
& (y \land x) \lor x \\
\iff & x
\end{align*}
\end{prop}

\subsection{Absorption of $\land$ over $\lor$}
\begin{prop}
\label{Proposition:land_lor_absorption_1}
\begin{align*}
& x \land (x \lor y) \\
\iff & x
\end{align*}
\end{prop}

\begin{prop}
\label{Proposition:land_lor_absorption_2}
\begin{align*}
& x \land (y \lor x) \\
\iff & x
\end{align*}
\end{prop}

\begin{prop}
\label{Proposition:land_lor_absorption_3}
\begin{align*}
& (x \lor y) \land x \\
\iff & x
\end{align*}
\end{prop}

\begin{prop}
\label{Proposition:land_lor_absorption_4}
\begin{align*}
& (y \lor x) \land x \\
\iff & x
\end{align*}
\end{prop}

\subsection{Distributivity of $\lor$ over $\land$}
\begin{prop}
\label{Proposition:lor_land_distributivity_1}
\begin{align*}
& x \lor (y \land z) \\
\iff & (x \lor y) \land (x \lor z)
\end{align*}
\end{prop}

\begin{prop}
\label{Proposition:lor_land_distributivity_2}
\begin{align*}
& (x \land y) \lor z \\
\iff & (x \lor z) \land (y \lor z)
\end{align*}
\end{prop}

\subsection{Distributivity of $\land$ over $\lor$}
\begin{prop}
\label{Proposition:land_lor_distributivity_1}
\begin{align*}
& x \land (y \lor z) \\
\iff & (x \land y) \lor (x \land z)
\end{align*}
\end{prop}

\begin{prop}
\label{Proposition:land_lor_distributivity_2}
\begin{align*}
& (x \lor y) \land z \\
\iff & (x \land z) \lor (y \land z)
\end{align*}
\end{prop}

\subsection{Double negation}
\begin{prop}
\label{Proposition:double_negation}
\begin{align*}
& \lnot (\lnot x) \\
\iff & x
\end{align*}
\end{prop}

\subsection{De Morgan's laws}
\begin{prop}
\label{Proposition:De_Morgan_lor}
\begin{align*}
& \lnot (x \lor y) \\
\iff & (\lnot x) \land (\lnot y)
\end{align*}
\end{prop}

\begin{prop}
\label{Proposition:De_Morgan_land}
\begin{align*}
& \lnot (x \land y) \\
\iff & (\lnot x) \lor (\lnot y)
\end{align*}
\end{prop}

\section{Basic Proposition}
\begin{prop}
\label{Proposition:x_lor_y_complement}
\begin{align*}
& (x \land (\lnot y)) \lor y \\
\iff & x \lor y
\end{align*}
Proof of Proposition \ref{Proposition:x_lor_y_complement}
\begin{align*}
& (x \land (\lnot y)) \lor y \\
\iff & (x \lor y) \land ((\lnot y) \lor y)
&& \text{Proposition \ref{Proposition:lor_land_distributivity_2}} \\
\iff & (x \lor y) \land (\text{True})
&& \text{Proposition \ref{Proposition:lor_complement_2}} \\
\iff & x \lor y
&& \text{Proposition \ref{Proposition:land_identity_1}} \\
\end{align*}
\end{prop}

\section{Proof technique}
\begin{prop}
\label{Proposition:true_statement}
\begin{align*}
& x \iff (\text{True}) \\
\iff & x
\end{align*}
Proof of Proposition \ref{Proposition:true_statement}
\begin{align*}
& x \iff (\text{True}) \\
\overset{\operatorname{def}}{\iff} & (x \land (\text{True})) \lor ((\lnot x) \land (\lnot (\text{True})))
&& \text{Definition \ref{Definition:iff}} \\
\overset{\operatorname{def}}{\iff} & (x \land (\text{True})) \lor ((\lnot x) \land (\text{False}))
&& \text{Definition \ref{Definition:lnot_True}} \\
\iff & x \lor ((\lnot x) \land (\text{False}))
&& \text{Proposition \ref{Proposition:land_identity_1}} \\
\iff & x \lor (\text{False})
&& \text{Proposition \ref{Proposition:land_annihilator_1}} \\
\iff & x
&& \text{Proposition \ref{Proposition:lor_identity_1}} \\
\end{align*}
\end{prop}

\begin{prop}
\label{Proposition:implies_lor}
\begin{align*}
& x \implies y \\
\implies & (x \lor z) \implies (y \lor z)
\end{align*}
Proof of Proposition \ref{Proposition:implies_lor}
\begin{align*}
& (x \implies y) \implies ((x \lor z) \implies (y \lor z)) \\
\overset{\operatorname{def}}{\iff} & ((\lnot x) \lor y) \implies ((x \lor z) \implies (y \lor z))
&& \text{Definition \ref{Definition:implies}} \\
\overset{\operatorname{def}}{\iff} & ((\lnot x) \lor y) \implies ((\lnot (x \lor z)) \lor (y \lor z))
&& \text{Definition \ref{Definition:implies}} \\
\overset{\operatorname{def}}{\iff} & (\lnot ((\lnot x) \lor y)) \lor ((\lnot (x \lor z)) \lor (y \lor z))
&& \text{Definition \ref{Definition:implies}} \\
\iff & ((\lnot (\lnot x)) \land (\lnot y)) \lor ((\lnot (x \lor z)) \lor (y \lor z))
&& \text{Proposition \ref{Proposition:De_Morgan_lor}} \\
\iff & (x \land (\lnot y)) \lor ((\lnot (x \lor z)) \lor (y \lor z))
&& \text{Proposition \ref{Proposition:double_negation}} \\
\iff & (x \land (\lnot y)) \lor (((\lnot x) \land (\lnot z)) \lor (y \lor z))
&& \text{Proposition \ref{Proposition:De_Morgan_lor}} \\
\iff & (x \land (\lnot y)) \lor (((\lnot x) \land (\lnot z)) \lor (z \lor y))
&& \text{Proposition \ref{Proposition:lor_commutativity}} \\
\iff & (x \land (\lnot y)) \lor ((((\lnot x) \land (\lnot z)) \lor z) \lor y)
&& \text{Proposition \ref{Proposition:lor_associativity}} \\
\iff & (x \land (\lnot y)) \lor (y \lor (((\lnot x) \land (\lnot z)) \lor z))
&& \text{Proposition \ref{Proposition:lor_commutativity}} \\
\iff & ((x \land (\lnot y)) \lor y) \lor (((\lnot x) \land (\lnot z)) \lor z)
&& \text{Proposition \ref{Proposition:lor_associativity}} \\
\iff & (x \lor y) \lor (((\lnot x) \land (\lnot z)) \lor z)
&& \text{Proposition \ref{Proposition:x_lor_y_complement}} \\
\iff & (x \lor y) \lor ((\lnot x) \lor z)
&& \text{Proposition \ref{Proposition:x_lor_y_complement}} \\
\iff & ((x \lor y) \lor (\lnot x)) \lor z
&& \text{Proposition \ref{Proposition:lor_associativity}} \\
\iff & ((\lnot x) \lor (x \lor y)) \lor z
&& \text{Proposition \ref{Proposition:lor_commutativity}} \\
\iff & (((\lnot x) \lor x) \lor y) \lor z
&& \text{Proposition \ref{Proposition:lor_associativity}} \\
\iff & ((\text{True}) \lor y) \lor z
&& \text{Proposition \ref{Proposition:lor_complement_2}} \\
\iff & (\text{True}) \lor z
&& \text{Proposition \ref{Proposition:lor_annihilator_2}} \\
\iff & \text{True}
&& \text{Proposition \ref{Proposition:lor_annihilator_2}} \\
\end{align*}
\end{prop}

\begin{prop}
\label{Proposition:implies_land}
\begin{align*}
(x \implies y) \implies ((x \land z) \implies (y \land z))
\end{align*}
\end{prop}

\begin{prop}
\label{Proposition:contrapositive}
Contrapositive
\begin{align*}
(x \implies y) \iff ((\lnot y) \implies (\lnot x))
\end{align*}
\end{prop}

\begin{prop}
\label{Proposition:implies_transitive}
Transitive property of $\implies$.
\begin{align*}
((x \implies y) \land (y \implies z)) \implies (x \implies z)
\end{align*}
\end{prop}

\begin{prop}
\begin{align*}
(x \iff y) \iff ((x \implies y) \land (y \implies x))
\end{align*}
\end{prop}

\begin{prop}
\label{Proposition:iff_lor}
\begin{align*}
(x \iff y) \implies ((x \lor z) \iff (y \lor z))
\end{align*}
\end{prop}

\begin{prop}
\label{Proposition:iff_land}
\begin{align*}
(x \iff y) \implies ((x \land z) \iff (y \land z))
\end{align*}
\end{prop}

\begin{prop}
\label{Proposition:iff_symmetric}
Symmetric property of $\iff$.
\begin{align*}
(x \iff y) \iff (y \iff x)
\end{align*}
\end{prop}

\begin{prop}
\label{Proposition:iff_lnot}
\begin{align*}
(x \iff y) \implies ((\lnot x) \iff (\lnot y))
\end{align*}
\end{prop}

\begin{prop}
\label{Proposition:iff_transitive}
Transitive property of $\iff$.
\begin{align*}
((x \iff y) \land (y \iff z)) \implies (x \iff z)
\end{align*}
\end{prop}

\begin{prop}
\label{Proposition:iff_reflexive}
Reflexive property of $\iff$.
\begin{align*}
& x \\
\iff & x
\end{align*}
Proof of Proposition \ref{Proposition:iff_reflexive}
\begin{align*}
& x \iff x \\
\overset{\operatorname{def}}{\iff} & (x \land x) \lor ((\lnot x) \land (\lnot x))
&& \text{Definition \ref{Definition:iff}} \\
\iff & x \lor ((\lnot x) \land (\lnot x))
&& \text{Proposition \ref{Proposition:land_idempotence}} \\
\iff & x \lor (\lnot x)
&& \text{Proposition \ref{Proposition:land_idempotence}} \\
\iff & \text{True}
&& \text{Proposition \ref{Proposition:lor_complement_1}} \\
\end{align*}
\end{prop}

\section{Quantifiers}
\begin{defn}
Universal quantifier is denoted by $\forall$.
\begin{align*}
& \forall x, P(x) \\
\overset{\operatorname{def}}{\iff} & (P(x_1) \land P(x_2) \land \dots)
\end{align*}
\end{defn}

\begin{defn}
Existential quantifier is denoted by $\exists$.
\begin{align*}
& \exists x, P(x) \\
\overset{\operatorname{def}}{\iff} & (P(x_1) \lor P(x_2) \lor \dots)
\end{align*}
\end{defn}

\begin{prop}
\label{Proposition:forall_land_commutativity}
\begin{align*}
(\forall x (P(x) \land Q(x))) \iff (\forall x, P(x)) \land (\forall x, Q(x))
\end{align*}
\end{prop}

\begin{prop}
\label{Proposition:exists_lor_commutativity}
\begin{align*}
(\exists x, P(x)) \lor (\exists x, Q(x)) \iff (\exists x, (P(x) \lor Q(x)))
\end{align*}
\end{prop}

\begin{prop}
\label{Proposition:lor_forall_distributivity}
\begin{align*}
(P \lor (\forall x, Q(x))) \iff (\forall x (P \lor Q(x)))
\end{align*}
\end{prop}

\begin{prop}
\label{Proposition:land_exists_distributivity}
\begin{align*}
(P \land (\exists x, Q(x))) \iff (\exists x (P \land Q(x)))
\end{align*}
\end{prop}

\begin{axm}
\label{Axiom:forall_independent_variable}
P does not depend on x.
\begin{align*}
(\forall x, P(y)) \iff P(y)
\end{align*}
\end{axm}

\begin{axm}
\label{Axiom:exists_independent_variable}
P does not depend on x.
\begin{align*}
(\exists x, P(y)) \iff P(y)
\end{align*}
\end{axm}

\begin{axm}
\label{Axiom:De_Morgan_1}
De Morgan's law
\begin{align*}
\lnot (\forall x, P(x)) \iff \exists x, \lnot (P(x))
\end{align*}
\end{axm}

\begin{axm}
\label{Axiom:De_Morgan_2}
De Morgan's law
\begin{align*}
\lnot (\exists x, P(x)) \iff \forall x, \lnot (P(x))
\end{align*}
\end{axm}

\begin{defn}
\label{Definition:uniqueness_quantifier}
Uniqueness quantifier is denoted by $!\exists$.
\begin{align*}
& !\exists x, P(x) \\
\overset{\operatorname{def}}{\iff} & (\exists x, P(x)) \land (\forall x \forall y (P(x) \land P(y) \implies x = y))
\end{align*}
\end{defn}

\begin{axm}
\label{Axiom:axiom_of_substitution}
Axiom of Substitution
\begin{align*}
\forall x( (\exists y((y = x) \land P(y))) \iff P(x) )
\end{align*}
\end{axm}

\section{Proposition}
\begin{prop}
\label{Proposition:land_implies_iff}
\begin{align*}
(P \land Q) \implies  (P \iff Q) \\
\end{align*}
\end{prop}

\begin{prop}
\label{Proposition:iff_contrapositive}
\begin{align*}
(\lnot P \iff \lnot Q) \iff (P \iff Q) \\
\end{align*}
\end{prop}

\begin{prop}
\label{Proposition:land_omit}
\begin{align*}
(P \land Q) \implies P \\
\end{align*}
\end{prop}

\begin{lemma}
\label{Lemma:uniqueness}
\begin{align*}
(P \land ((Q \land P) \implies R)) \implies (Q \implies R) \\
\end{align*}
\end{lemma}

\begin{prop}
\label{Proposition:implies_satisfy}
\begin{align*}
(P \land (P \implies Q)) \implies Q \\
\end{align*}
\end{prop}

\begin{prop}
\label{Proposition:iff_satisfy}
\begin{align*}
(P \land (P \iff Q)) \implies Q \\
\end{align*}
\end{prop}