\chapter{Set theory}
Set theory have one primitive notion, called set, and one binary relation, called set membership, denoted by $\in$.

\begin{defn}
Definition of $\notin$.
\begin{align*}
& A \notin B \\
\iff & \lnot (A \in B) \\
\end{align*}
\end{defn}

\begin{defn}
\label{Definition:universal_quantifier_in_set}
\begin{align*}
& \forall x \in S, P(x) \\
\iff & \forall x (x \in S \implies P(x))
\end{align*}
\end{defn}

\begin{defn}
\label{Definition:existential_quantifier_in_set}
\begin{align*}
& \exists x \in S, P(x) \\
\iff & \exists x (x \in S \land P(x))
\end{align*}
\end{defn}

\begin{prop}
\begin{align*}
\lnot (\forall x \in S, P(x)) \iff \exists x \in S, \lnot (P(x))
\end{align*} 
Proof: \\ \\
\begin{align*}
& \lnot (\forall x \in S, P(x)) \\
\iff & \lnot ( \forall x (x \in S \implies P(x)) )
&& \text{Definition \ref{Definition:universal_quantifier_in_set}} \\
\iff & \lnot ( \forall x (\lnot(x \in S) \lor P(x)) )
&& \text{Definition \ref{Definition:implies}} \\
\iff & \exists x, \lnot (\lnot(x \in S) \lor P(x))
&& \text{Axiom \ref{axiom:De_Morgan_1}} \\
\iff & \exists x, \lnot (\lnot(x \in S)) \land \lnot (P(x))
&& \text{Proposition \ref{Proposition:De_Morgan_2}} \\
\iff & \exists x, x \in S \land \lnot (P(x))
&& \text{Proposition \ref{Proposition:double_negation}} \\
\iff & \exists x \in S, \lnot (P(x))
&& \text{Definition \ref{Definition:existential_quantifier_in_set}} \\
\end{align*}
\end{prop}

\begin{prop}
\begin{align*}
\lnot (\exists x \in S, P(x)) \iff \forall x \in S, \lnot (P(x))
\end{align*} 
Proof: \\ \\
\begin{align*}
& \lnot (\exists x \in S, P(x)) \\
\iff & \lnot ( \exists x (x \in S \land P(x)) )
&& \text{Definition \ref{Definition:existential_quantifier_in_set}} \\
\iff & \forall x, \lnot (x \in S \land P(x))
&& \text{Axiom \ref{axiom:De_Morgan_2}} \\
\iff & \forall x, (\lnot(x \in S)) \lor (\lnot (P(x))
&& \text{Proposition \ref{Proposition:De_Morgan_1}} \\
\iff & \forall x, x \in S \implies \lnot (P(x))
&& \text{Definition \ref{Definition:implies}} \\
\iff & \forall x \in S, \lnot (P(x))
&& \text{Definition \ref{Definition:universal_quantifier_in_set}} \\
\end{align*}
\end{prop}

\section{Equality of sets}
\begin{defn}
\label{Definition:equality}
Definition of $=$.
\begin{align*}
& A = B \\
\iff & \forall x (x \in A \iff x \in B) \\
\end{align*}
\end{defn}

\begin{defn}
Definition of $\neq$.
\begin{align*}
& A \neq B \\
\iff & \lnot (A = B) \\
\end{align*}
\end{defn}

\begin{prop}
Reflexive property of equality
\begin{align*}
\forall x (x = x)
\end{align*}
Proof:
\begin{align*}
& \forall x ( \\
& \quad &&  && x = x \\
& \quad && \iff && \forall y (y \in x \iff y \in x)
&& \text{Definition \ref{Definition:equality}} \\
& \quad && \iff && \text{True}
&& \text{Proposition \ref{Proposition:iff_reflexive}} \\
& )
\end{align*}
\end{prop}

\begin{prop}
Symmetric property of equality
\begin{align*}
\forall x \forall y ((x = y) \implies (y=x))
\end{align*}
Proof:
\begin{align*}
& \forall x \forall y ( \\
& \quad &&  &&  x = y \\
& \quad && \implies &&  \forall z (z \in x \iff z \in y)
&& \text{Definition \ref{Definition:equality}} \\
& \quad && \implies &&  \forall z (z \in y \iff z \in x)
&& \text{Proposition \ref{Proposition:iff_symmetric}} \\
& \quad && \implies && y = x
&& \text{Definition \ref{Definition:equality}} \\
& )
\end{align*}
\end{prop}

\begin{prop}
Transitive property of equality
\begin{align*}
\forall x \forall y \forall z ((x = y) \land (y=z) \implies (x=z))
\end{align*}
Proof:
\begin{align*}
& \forall x \forall y \forall z ( \\
& \quad &&  &&  (x = y) \land (y=z) \\
& \quad && \implies && ( \forall w (w \in x \iff w \in y)) \land ( \forall w (w \in y \iff w \in z))
&& \text{Definition \ref{Definition:equality}} \\
& \quad && \implies && \forall w ((w \in x \iff w \in y) \land (w \in y \iff w \in z))
&& \text{Axiom \ref{axiom:forall_land_distributive}} \\
& \quad && \implies && \forall w (w \in x \iff w \in z)
&& \text{Proposition \ref{Proposition:iff_Transitive}} \\
& \quad && \implies && x = z
&& \text{Definition \ref{Definition:equality}} \\
& )
\end{align*}
\end{prop}

\begin{axm}
Axiom of Substitution
\begin{align*}
& \forall x \forall y ( \\
& x = y \implies \forall A (x \in A  \iff y \in A) \\
& )
\end{align*}
\end{axm}
